---
title: "Solution 4"
author: "Ben White"
date: "2/15/2018"
output: pdf_document
---

1. (1 point) For $0 < y < 1$: $$F_Y(y) = P(Y \leq y) = P(F_X(X) \leq y)= P(F_X^{-1}(F_X(X)) \leq F_X^{-1}(y))$$ $$= P(X \leq F_X^{-1}(y))= F_X(F_X^{-1}(y))= y.$$ This is the cdf of a standard uniform random variable.

1. (1 point per part)
    a. This transformation is monotonically decreasing. The inverse mapping is the function $g^{-1}(y) = e^{-y}$, which is differentiable. $\frac{d}{dy} g^{-1}(y) = -e^{-y},$ so the pdf of $Y$ is $f_Y(y) = f_X(e^{-y})|-e^{-y}| = e^{-y}$ if $y > 0$, and 0 otherwise. Note that $Y \sim \text{exponential}(1)$.

    
    b. $g(x) = x^3$ is a monotone transformation, with $g^{-1}(y) = y^{1/3}$ and $\frac{d}{dy}g^{-1}(y) = \frac{1}{3}y^{-2/3}$. So the pdf of $Y$ is $f_Y(y) = 42y^{5/3}(1 - y^{1/3})(\frac{1}{3}y^{-2/3}) = 14y(1 - y^{1/3}).$   
    
1. (1 point) We can find the pmf directly: $$f_Y(y) = P(Y = y)$$ $$=P(n-X = y)$$ $$=P(X = n-y)$$ $$=f_X(n-y)$$ $$= \frac{n!}{(n-y)!(n-(n-y))!}p^{n-y}(1 - p)^{n - (n-y)}$$ $$= \frac{n!}{(n-y)!y!}(1-p)^y(1 - (1-p))^{n-y}$$ We can see that $Y\sim \text{binom}(n, 1-p)$.

1. We can see that the support of $Y$ will be the real numbers between 0 and 1.
    a. (1 point) $$F_Y(y) = P(Y \leq y) = P(X^2 \leq y) = P(-\sqrt{y} \leq X \leq \sqrt{y}) = F_X(\sqrt{y}) - F_X(-\sqrt{y})$$ Differentiating to get the pdf: $$f_Y(y) = \frac{d}{dy}F_Y(y)$$ $$= \frac{d}{dy}[F_X(\sqrt{y}) - F_X(-\sqrt{y})]$$ $$=\frac{1}{2}y^{-1/2}f_X(\sqrt{y}) -  (-1)\frac{1}{2}y^{-1/2}f_X(-\sqrt{y})$$ $$\frac{1}{2\sqrt{y}}\left(\frac{1}{2}(1 + \sqrt{y}) + \frac{1}{2}(1 - \sqrt{y})\right)$$ $$=\frac{1}{2\sqrt{y}}$$ for $0 \leq y \leq 1$.
    
    b. (1 point) $$E[Y] = \int_{-\infty}^\infty yf_Y(y)dy = \int_0^1 \frac{y}{2\sqrt{y}}dy = \int_0^1 \frac{\sqrt{y}}{2} dy = \frac{1}{3}$$
  
    c. (1 point) $$E[Y^2] = \int_{-\infty}^\infty y^2 f_Y(y) dy = \int_0^1 \frac{y^2}{2\sqrt{y}}dy = \int_0^1 \frac{y^{3/2}}{2} dy = \frac{1}{5}$$ $$\text{Var}(Y) = E[Y^2] - (E[Y])^2 = \frac{1}{5} - \frac{1^2}{3^2} = \frac{4}{45}$$
  
1. We can see that the support of $Y$ will be the non-negative real numbers.
    a. (1 point) $$F_Y(y) = P(Y \leq y) = P(|X| \leq y) = P(-y \leq X \leq y) = F_X(y) - F_X(-y)$$ Differentiating to get the pdf: $$f_Y(y) = \frac{d}{dy}F_Y(y)$$ $$= (1)f_X(y) - (-1)f_X(y)$$ $$=2f_X(x)$$ $$= \sqrt{\frac{2}{\pi}}e^{-y^2/2}$$ for $y \geq 0$
    
    b. (1 point) $$E[Y] = \int_{-\infty}^\infty yf_Y(y)dy = \int_0^\infty y \sqrt{\frac{2}{\pi}}e^{-y^2/2} dy = \sqrt{\frac{2}{\pi}}$$
  
    c. (1 point) $$E[Y^2] = \int_{-\infty}^\infty y^2f_Y(y)dy = \int_0^\infty y^2 \sqrt{\frac{2}{\pi}}e^{-y^2/2} dy = 1$$ $$\text{Var}(Y) = E[Y^2] - (E[Y])^2 = 1 - \frac{2}{\pi}$$

    
    